calculations for lambda calculi without arithmetic

LambdaCBNameArith.v
@@ -1,6 +1,6 @@
 (** Calculation of an abstract machine for the call-by-name lambda
-calculus. The resulting abstract machine coincides with the Krivine
-machine. *)
+calculus + arithmetic. The resulting abstract machine coincides with
+the Krivine machine (extended with arithmetic). *)
 
 Require Import List.
 Require Import ListIndex.
@@ -9,6 +9,8 @@ Require Import Tactics.
 (** * Syntax *)
 
 Inductive Expr : Set := 
+| Val : nat -> Expr 
+| Add : Expr -> Expr -> Expr
 | Var : nat -> Expr
 | Abs : Expr -> Expr
 | App : Expr -> Expr -> Expr.
@@ -22,10 +24,14 @@ abstract machines" (we use Haskell syntax to describe the evaluator):
 <<
 type Env   = [Thunk]
 data Thunk = Thunk (() -> Value)
-data Value = Clo (Thunk -> Value)
+data Value = Num Int | Clo (Thunk -> Value)
 
 
 eval :: Expr -> Env -> Value
+eval (Val n)   e = Num n
+eval (Add x y) e = case eval x e of
+                     Num n -> case eval y e of
+                                Num m -> Num (n + m)
 eval (Var i)   e = case e !! i of
                      Thunk t -> t ()
 eval (Abs x)   e = Clo (\t -> eval x (t : e))
@@ -41,11 +47,14 @@ Inductive Thunk : Set  :=
 Definition Env : Set := list Thunk.
 
 Inductive Value : Set :=
+| Num : nat -> Value
 | Clo : Expr -> Env -> Value.
 
 Reserved Notation "x ⇓[ e ] y" (at level 80, no associativity).
 
 Inductive eval : Expr -> Env -> Value -> Prop :=
+| eval_val e n : Val n ⇓[e] Num n
+| eval_add e x y m n : x ⇓[e] Num n -> y ⇓[e] Num m -> Add x y ⇓[e] Num (n + m)
 | eval_var e e' x i v : nth e i = Some (thunk x e') -> x ⇓[e'] v -> Var i ⇓[e] v
 | eval_abs e x : Abs x ⇓[e] Clo x e
 | eval_app e e' x x' v y  : x ⇓[e] Clo x' e' -> x' ⇓[thunk y e :: e'] v -> App x y ⇓[e] v
@@ -54,6 +63,8 @@ where "x ⇓[ e ] y" := (eval x e y).
 (** * Abstract machine *)
 
 Inductive CONT : Set :=
+| NEXT : Expr -> Env -> CONT -> CONT
+| ADD : CONT -> nat -> CONT
 | APP : Expr -> Env -> CONT -> CONT
 | HALT : CONT
 .
@@ -71,9 +82,13 @@ Notation "⟪ c , v ⟫" := (apply c v).
 
 Reserved Notation "x ==> y" (at level 80, no associativity).
 Inductive AM : Conf -> Conf -> Prop :=
+| am_val n e c : ⟨Val n, e, c⟩ ==> ⟪c, Num n⟫
+| am_add x y e c : ⟨Add x y, e, c⟩ ==> ⟨x, e, NEXT y e c⟩
 | am_var i e c x e' : nth e i = Some (thunk x e') -> ⟨Var i, e, c⟩ ==> ⟨x, e', c⟩
 | am_abs x e c : ⟨Abs x, e, c⟩ ==> ⟪c, Clo x e⟫
 | am_app x y e c : ⟨App x y, e, c⟩ ==> ⟨x, e, APP y e c⟩
+| am_NEXT y e c n : ⟪NEXT y e c, Num n⟫ ==> ⟨y, e, ADD c n⟩
+| am_ADD c n m : ⟪ADD c n, Num m⟫ ==> ⟪c, Num (n+m)⟫
 | am_APP y e c x' e' : ⟪APP y e c, Clo x' e'⟫ ==> ⟨x', thunk y e::e', c⟩
 where "x ==> y" := (AM x y).
 
@@ -101,6 +116,30 @@ Proof.
   induction H;intros.
 
 (** Calculation of the abstract machine *)
+
+(** - [Val n ⇓[e] Num n]: *)
+
+  begin
+  ⟪c, Num n⟫.
+  <== { apply am_val }
+  ⟨Val n, e, c⟩.
+  [].
+
+(** - [Add x y ⇓[e] Num (n + m)]: *)
+
+  begin
+    ⟪c, Num (n + m)⟫.
+  <== { apply am_ADD }
+      ⟪ADD c n, Num m⟫.
+  <<= { apply IHeval2 }
+      ⟨y, e, ADD c n⟩.
+  <== { apply am_NEXT }
+      ⟪NEXT y e c, Num n⟫.
+  <<= { apply IHeval1 }
+      ⟨x, e, NEXT y e c⟩.
+  <== {apply am_add}
+      ⟨Add x y, e, c ⟩.
+  [].
 
 (** - [Var i ⇓[e] v] *)
 
