LambdaCBV.v
@@ -1,6 +1,6 @@
 (** Calculation of an abstract machine for the call-by-value lambda
-calculus + arithmetic. The resulting abstract machine coincides with
-the CEK machine (extended with arithmetic). *)
+calculus. The resulting abstract machine coincides with the CEK
+machine. *)
 
 Require Import List.
 Require Import ListIndex.
@@ -9,26 +9,18 @@ Require Import Tactics.
 (** * Syntax *)
 
 Inductive Expr : Set := 
-| Val : nat -> Expr 
-| Add : Expr -> Expr -> Expr
 | Var : nat -> Expr
 | Abs : Expr -> Expr
 | App : Expr -> Expr -> Expr.
 
 (** * Semantics *)
 
-(** The evaluator for this language is given as follows (as in the
-paper):
+(** The evaluator for this language is given as follows:
 <<
 type Env = [Value]
-data Value =  Num Int | Fun (Value -> Value)
-
+data Value =  Fun (Value -> Value)
 
 eval ::  Expr -> Env -> Value
-eval (Val n) e   = Num n
-eval (Add x y) e = case eval x e of
-                     Num n -> case eval y e of
-                                Num m -> Num (n+m)
 eval (Var i) e   = e !! i
 eval (Abs x) e   = Fun (\v -> eval x (v:e))
 eval (App x y) e = case eval x e of
@@ -38,7 +30,6 @@ After defunctionalisation and translation into relational form we
 obtain the semantics below. *)
 
 Inductive Value : Set :=
-| Num : nat -> Value
 | Clo : Expr -> list Value -> Value.
 
 Definition Env := list Value.
@@ -46,8 +37,6 @@ Definition Env := list Value.
 Reserved Notation "x ⇓[ e ] y" (at level 80, no associativity).
 
 Inductive eval : Expr -> Env -> Value -> Prop :=
-| eval_val e n : Val n ⇓[e] Num n
-| eval_add e x y m n : x ⇓[e] Num n -> y ⇓[e] Num m -> Add x y ⇓[e] Num (n + m)
 | eval_var e i v : nth e i = Some v -> Var i ⇓[e] v
 | eval_abs e x : Abs x ⇓[e] Clo x e
 | eval_app e e' x x' w y v : x ⇓[e] Clo x' e' -> y ⇓[e] v -> x' ⇓[v :: e'] w -> App x y ⇓[e] w
@@ -56,8 +45,6 @@ where "x ⇓[ e ] y" := (eval x e y).
 (** * Abstract machine *)
 
 Inductive CONT : Set :=
-| NEXT : Expr -> Env -> CONT -> CONT
-| ADD : CONT -> nat -> CONT
 | FUN : Expr -> Env -> CONT -> CONT
 | ARG : Expr -> Env -> CONT -> CONT
 | HALT : CONT
@@ -76,13 +63,9 @@ Notation "⟪ c , v ⟫" := (apply c v).
 
 Reserved Notation "x ==> y" (at level 80, no associativity).
 Inductive AM : Conf -> Conf -> Prop :=
-| am_val n e c : ⟨Val n, e, c⟩ ==> ⟪c, Num n⟫
-| am_add x y e c : ⟨Add x y, e, c⟩ ==> ⟨x, e, NEXT y e c⟩
 | am_var i e c v : nth e i = Some v -> ⟨Var i, e, c⟩ ==> ⟪c, v⟫
 | am_abs x e c : ⟨Abs x, e, c⟩ ==> ⟪c, Clo x e⟫
 | am_app x y e c : ⟨App x y, e, c⟩ ==> ⟨x, e, ARG y e c⟩
-| am_NEXT y e c n : ⟪NEXT y e c, Num n⟫ ==> ⟨y, e, ADD c n⟩
-| am_ADD c n m : ⟪ADD c n, Num m⟫ ==> ⟪c, Num (n+m)⟫
 | am_FUN x' e' c v : ⟪FUN x' e' c, v⟫ ==> ⟨x', v::e', c⟩
 | am_ARG y e c x' e' : ⟪ARG y e c, Clo x' e'⟫ ==> ⟨y, e, FUN x' e' c⟩
 where "x ==> y" := (AM x y).
@@ -112,29 +95,6 @@ Proof.
 
 (** Calculation of the abstract machine *)
 
-(** - [Val n ⇓[e] Num n]: *)
-
-  begin
-  ⟪c, Num n⟫.
-  <== { apply am_val }
-  ⟨Val n, e, c⟩.
-  [].
-
-(** - [Add x y ⇓[e] Num (n + m)]: *)
-
-  begin
-    ⟪c, Num (n + m)⟫.
-  <== { apply am_ADD }
-      ⟪ADD c n, Num m⟫.
-  <<= { apply IHeval2 }
-      ⟨y, e, ADD c n⟩.
-  <== { apply am_NEXT }
-      ⟪NEXT y e c, Num n⟫.
-  <<= { apply IHeval1 }
-      ⟨x, e, NEXT y e c⟩.
-  <== {apply am_add}
-      ⟨Add x y, e, c ⟩.
-  [].
 
 (** - [Var i ⇓[e] v] *)
 
