LambdaCBVArith.v
@@ -1,0 +1,191 @@
+(** Calculation of an abstract machine for the call-by-value lambda
+calculus + arithmetic. The resulting abstract machine coincides with
+the CEK machine (extended with arithmetic). *)
+
+Require Import List.
+Require Import ListIndex.
+Require Import Tactics.
+
+(** * Syntax *)
+
+Inductive Expr : Set := 
+| Val : nat -> Expr 
+| Add : Expr -> Expr -> Expr
+| Var : nat -> Expr
+| Abs : Expr -> Expr
+| App : Expr -> Expr -> Expr.
+
+(** * Semantics *)
+
+(** The evaluator for this language is given as follows:
+<<
+type Env = [Value]
+data Value =  Num Int | Fun (Value -> Value)
+
+
+eval ::  Expr -> Env -> Value
+eval (Val n) e   = Num n
+eval (Add x y) e = case eval x e of
+                     Num n -> case eval y e of
+                                Num m -> Num (n+m)
+eval (Var i) e   = e !! i
+eval (Abs x) e   = Fun (\v -> eval x (v:e))
+eval (App x y) e = case eval x e of
+                     Fun f -> f (eval y e)
+>>
+After defunctionalisation and translation into relational form we
+obtain the semantics below. *)
+
+Inductive Value : Set :=
+| Num : nat -> Value
+| Clo : Expr -> list Value -> Value.
+
+Definition Env := list Value.
+
+Reserved Notation "x ⇓[ e ] y" (at level 80, no associativity).
+
+Inductive eval : Expr -> Env -> Value -> Prop :=
+| eval_val e n : Val n ⇓[e] Num n
+| eval_add e x y m n : x ⇓[e] Num n -> y ⇓[e] Num m -> Add x y ⇓[e] Num (n + m)
+| eval_var e i v : nth e i = Some v -> Var i ⇓[e] v
+| eval_abs e x : Abs x ⇓[e] Clo x e
+| eval_app e e' x x' w y v : x ⇓[e] Clo x' e' -> y ⇓[e] v -> x' ⇓[v :: e'] w -> App x y ⇓[e] w
+where "x ⇓[ e ] y" := (eval x e y).
+
+(** * Abstract machine *)
+
+Inductive CONT : Set :=
+| NEXT : Expr -> Env -> CONT -> CONT
+| ADD : CONT -> nat -> CONT
+| FUN : Expr -> Env -> CONT -> CONT
+| ARG : Expr -> Env -> CONT -> CONT
+| HALT : CONT
+.
+
+(** * Virtual Machine *)
+
+Inductive Conf : Set := 
+| eval'' : Expr -> Env -> CONT -> Conf
+| apply : CONT -> Value -> Conf.
+
+Notation "⟨ x , e , c ⟩" := (eval'' x e c).
+Notation "⟪ c , v ⟫" := (apply c v).
+
+
+
+Reserved Notation "x ==> y" (at level 80, no associativity).
+Inductive AM : Conf -> Conf -> Prop :=
+| am_val n e c : ⟨Val n, e, c⟩ ==> ⟪c, Num n⟫
+| am_add x y e c : ⟨Add x y, e, c⟩ ==> ⟨x, e, NEXT y e c⟩
+| am_var i e c v : nth e i = Some v -> ⟨Var i, e, c⟩ ==> ⟪c, v⟫
+| am_abs x e c : ⟨Abs x, e, c⟩ ==> ⟪c, Clo x e⟫
+| am_app x y e c : ⟨App x y, e, c⟩ ==> ⟨x, e, ARG y e c⟩
+| am_NEXT y e c n : ⟪NEXT y e c, Num n⟫ ==> ⟨y, e, ADD c n⟩
+| am_ADD c n m : ⟪ADD c n, Num m⟫ ==> ⟪c, Num (n+m)⟫
+| am_FUN x' e' c v : ⟪FUN x' e' c, v⟫ ==> ⟨x', v::e', c⟩
+| am_ARG y e c x' e' : ⟪ARG y e c, Clo x' e'⟫ ==> ⟨y, e, FUN x' e' c⟩
+where "x ==> y" := (AM x y).
+
+
+(** * Calculation *)
+
+(** Boilerplate to import calculation tactics *)
+
+Module AM <: Preorder.
+Definition Conf := Conf.
+Definition VM := AM.
+End AM.
+Module AMCalc := Calculation AM.
+Import AMCalc.
+
+(** Specification of the abstract machine *)
+
+Theorem spec x e r c : x ⇓[e] r -> ⟨x, e, c⟩ =>> ⟪c, r⟫.
+
+(** Setup the induction proof *)
+
+Proof.
+  intros.
+  generalize dependent c.
+  induction H;intros.
+
+(** Calculation of the abstract machine *)
+
+(** - [Val n ⇓[e] Num n]: *)
+
+  begin
+  ⟪c, Num n⟫.
+  <== { apply am_val }
+  ⟨Val n, e, c⟩.
+  [].
+
+(** - [Add x y ⇓[e] Num (n + m)]: *)
+
+  begin
+    ⟪c, Num (n + m)⟫.
+  <== { apply am_ADD }
+      ⟪ADD c n, Num m⟫.
+  <<= { apply IHeval2 }
+      ⟨y, e, ADD c n⟩.
+  <== { apply am_NEXT }
+      ⟪NEXT y e c, Num n⟫.
+  <<= { apply IHeval1 }
+      ⟨x, e, NEXT y e c⟩.
+  <== {apply am_add}
+      ⟨Add x y, e, c ⟩.
+  [].
+
+(** - [Var i ⇓[e] v] *)
+
+  begin
+    ⟪c, v ⟫.
+  <== {apply am_var}
+    ⟨Var i, e, c ⟩.
+   [].
+
+(** - [Abs x ⇓[e] Clo x e] *)
+
+  begin
+    ⟪c, Clo x e⟫.
+  <== { apply am_abs }
+    ⟨Abs x, e, c⟩.
+  [].
+
+(** - [App x y ⇓[e] w] *)
+
+  begin
+    ⟪c, w⟫.
+  <<= { apply IHeval3 }
+    ⟨x', (v::e'), c⟩.
+  <== { apply am_FUN }
+    ⟪FUN x' e' c, v⟫.
+  <<= {apply IHeval2}
+    ⟨y, e, FUN x' e' c⟩.
+  <== {apply am_ARG}
+    ⟪ARG y e c, Clo x' e'⟫.
+  <<= {apply IHeval1}
+    ⟨x, e, ARG y e c⟩.
+  <== {apply am_app}
+    ⟨App x y, e, c⟩.
+  [].
+Qed.
+  
+(** * Soundness *)
+
+Lemma determ_am : determ AM.
+  intros C c1 c2 V. induction V; intro V'; inversion V'; subst; congruence.
+Qed.
+  
+
+Definition terminates (p : Expr) : Prop := exists r, p ⇓[nil] r.
+
+Theorem sound x C : terminates x -> ⟨x, nil, HALT⟩ =>>! C -> 
+                          exists r, C = ⟪HALT, r⟫ /\ x ⇓[nil] r.
+Proof.
+  unfold terminates. intros. destruct H as [r T].
+  
+  pose (spec x nil r HALT) as H'. exists r. split. pose (determ_trc determ_am) as D.
+  unfold determ in D. eapply D. eassumption. split. eauto. intro. destruct H. 
+  inversion H. assumption.
+Qed.
+  
